books/centaur/vl/mlib/immdeps.lisp
@@ -32,6 +32,7 @@
 (include-book "scopestack")
 (include-book "hid-tools")
 (include-book "reportcard")
+(include-book "centaur/fty/visitor" :dir :system)
 (include-book "centaur/depgraph/mergesort-alist-values" :dir :system)
 (local (include-book "../util/arithmetic"))
 (local (std::add-default-post-define-hook :fix))
@@ -237,7 +238,7 @@ that package.</li>
 elements.")
 
 (local (xdoc::set-default-parents immdeps-main))
-(define vl-scopeexpr-immdeps
+(define vl-scopeexpr-top-immdeps
   ((x vl-scopeexpr-p)
    (ans vl-immdeps-p)
    &key
@@ -258,36 +259,116 @@ elements.")
       ;; or we might want to just not support it.
       (vl-immdeps-fix ans))))
 
+;; (defines vl-expr-immdeps
+;;   :verify-guards nil
+;;   (define vl-expr-immdeps
+;;     ((x vl-expr-p)
+;;      (ans vl-immdeps-p)
+;;      &key
+;;      ((ss  vl-scopestack-p  "Our current scope.") 'ss)
+;;      ((ctx acl2::any-p      "Context for warnings.") 'ctx))
+;;     :measure (vl-expr-count x)
+;;     :returns (ans vl-immdeps-p)
+;;     (b* ((ans (vl-expr-case x
+;;                 :vl-index (vl-scopeexpr-immdeps x.scope ans)
+;;                 :otherwise ans)))
+;;       (vl-exprlist-immdeps (vl-expr->subexprs x) ans)))
 
-(defines vl-expr-immdeps
-  :verify-guards nil
-  (define vl-expr-immdeps
-    ((x vl-expr-p)
-     (ans vl-immdeps-p)
-     &key
-     ((ss  vl-scopestack-p  "Our current scope.") 'ss)
-     ((ctx acl2::any-p      "Context for warnings.") 'ctx))
-    :measure (vl-expr-count x)
-    :returns (ans vl-immdeps-p)
-    (b* ((ans (vl-expr-case x
-                :vl-index (vl-scopeexpr-immdeps x.scope ans)
-                :otherwise ans)))
-      (vl-exprlist-immdeps (vl-expr->subexprs x) ans)))
+;;   (define vl-exprlist-immdeps
+;;     ((x vl-exprlist-p)
+;;      (ans vl-immdeps-p)
+;;      &key
+;;      ((ss  vl-scopestack-p  "Our current scope.") 'ss)
+;;      ((ctx acl2::any-p      "Context for warnings.") 'ctx))
+;;     :measure (vl-exprlist-count x)
+;;     :returns (ans vl-immdeps-p)
+;;     (if (atom x)
+;;         (vl-immdeps-fix ans)
+;;       (vl-exprlist-immdeps (cdr x) (vl-expr-immdeps (car x) ans))))
+;;   ///
+;;   (verify-guards vl-expr-immdeps-fn)
+;;   (deffixequiv-mutual vl-expr-immdeps))
 
-  (define vl-exprlist-immdeps
-    ((x vl-exprlist-p)
-     (ans vl-immdeps-p)
-     &key
-     ((ss  vl-scopestack-p  "Our current scope.") 'ss)
-     ((ctx acl2::any-p      "Context for warnings.") 'ctx))
-    :measure (vl-exprlist-count x)
-    :returns (ans vl-immdeps-p)
-    (if (atom x)
-        (vl-immdeps-fix ans)
-      (vl-exprlist-immdeps (cdr x) (vl-expr-immdeps (car x) ans))))
-  ///
-  (verify-guards vl-expr-immdeps-fn)
-  (deffixequiv-mutual vl-expr-immdeps))
+
+(fty::defvisitor-template immdeps ((x :object)
+                                   (ans vl-immdeps-p)
+                                   &key
+                                   ((ss vl-scopestack-p) 'ss)
+                                   ((ctx acl2::any-p) 'ctx))
+  :returns (ans1 (:acc ans :fix (vl-immdeps-fix ans)) vl-immdeps-p)
+  :field-fns ((atts :skip))
+  :prod-fns ((vl-special     (type :skip))
+             (vl-value       (type :skip))
+             (vl-index       (type :skip))
+             (vl-unary       (type :skip))
+             (vl-binary      (type :skip))
+             (vl-qmark       (type :skip))
+             (vl-mintypmax   (type :skip))
+             (vl-concat      (type :skip))
+             (vl-multiconcat (type :skip))
+             (vl-call        (type :skip))
+             (vl-cast        (type :skip))
+             (vl-inside      (type :skip))
+             (vl-tagged      (type :skip))
+             (vl-pattern     (type :skip)))
+  :fnname-template <type>-immdeps)
+
+;; Not dealing with anything that might add a scope yet.
+(fty::defvisitor vl-expr-immdeps
+  :template immdeps
+  :type expressions-and-datatypes
+  :type-fns ((vl-scopeexpr vl-scopeexpr-immdeps-fn))
+  :renames ((vl-scopeexpr vl-scopeexpr-immdeps-aux))
+  :measure (two-nats-measure :count 0)
+  (define vl-scopeexpr-immdeps ((x vl-scopeexpr-p)
+                                (ans vl-immdeps-p)
+                                &key
+                                ((ss vl-scopestack-p) 'ss)
+                                ((ctx acl2::any-p) 'ctx))
+    :returns (ans1 vl-immdeps-p)
+    :measure (two-nats-measure (vl-scopeexpr-count x) 1)
+    (vl-scopeexpr-immdeps-aux x (vl-scopeexpr-top-immdeps x ans))))
+
+(fty::defvisitors vl-misc-immdeps
+  :template immdeps
+  :types (vl-maybe-gatedelay
+          vl-arguments
+          vl-paramargs
+          vl-paramtype
+          vl-maybe-delayoreventcontrol))
+
+  
+
+
+
+(fty::defvisitor vl-stmt-immdeps
+  :type statements
+  :template immdeps
+  :type-fns ((vl-stmt vl-stmt-immdeps-fn))
+  :renames ((vl-stmt vl-stmt-immdeps-aux))
+  :measure (two-nats-measure :count 0)
+  (define vl-stmt-immdeps ((x vl-stmt-p)
+                           (ans vl-immdeps-p)
+                           &key
+                           ((ss vl-scopestack-p) 'ss)
+                           ((ctx acl2::any-p) 'ctx))
+    :returns (ans1 vl-immdeps-p)
+    :measure (two-nats-measure (vl-stmt-count x) 1)
+    (b* ((ss (vl-stmt-case x
+               :vl-blockstmt (vl-scopestack-push (vl-blockstmt->blockscope x) ss)
+               :otherwise ss)))
+      (vl-stmt-immdeps-aux x ans))))
+
+
+;; (fty::defvisitor-template immdeps-no-ctx ((x :object)
+;;                                           (ans vl-immdeps-p)
+;;                                           &key
+;;                                           ((ss vl-scopestack-p) 'ss))
+;;   :wrapper (b* ((?ctx x)) :body)
+  
+
+
+
 
 (defmacro def-vl-immdeps (type &key body verbosep guard-debug prepwork (ctxp 't))
   (let* ((mksym-package-symbol 'vl::foo)
@@ -326,143 +407,143 @@ elements.")
             (ans (,element-collect (car x) ans)))
          (,list-collect (cdr x) ans)))))
 
-(def-vl-immdeps vl-maybe-expr
-  :body
-  (if x
-      (vl-expr-immdeps x ans)
-    ans))
+;; (def-vl-immdeps vl-maybe-expr
+;;   :body
+;;   (if x
+;;       (vl-expr-immdeps x ans)
+;;     ans))
 
-(def-vl-immdeps vl-range
-  :body
-  (b* (((vl-range x) x)
-       (ans (vl-expr-immdeps x.msb ans))
-       (ans (vl-expr-immdeps x.lsb ans)))
-    ans))
+;; (def-vl-immdeps vl-range
+;;   :body
+;;   (b* (((vl-range x) x)
+;;        (ans (vl-expr-immdeps x.msb ans))
+;;        (ans (vl-expr-immdeps x.lsb ans)))
+;;     ans))
 
-(def-vl-immdeps vl-maybe-range
-  :body
-  (if x
-      (vl-range-immdeps x ans)
-    ans))
+;; (def-vl-immdeps vl-maybe-range
+;;   :body
+;;   (if x
+;;       (vl-range-immdeps x ans)
+;;     ans))
 
-(def-vl-immdeps-list vl-rangelist vl-range)
+;; (def-vl-immdeps-list vl-rangelist vl-range)
 
-(def-vl-immdeps vl-packeddimension
-  :body
-  (vl-packeddimension-case x
-    :unsized ans
-    :range (vl-range-immdeps x.range ans)))
+;; (def-vl-immdeps vl-packeddimension
+;;   :body
+;;   (vl-packeddimension-case x
+;;     :unsized ans
+;;     :range (vl-range-immdeps x.range ans)))
 
-(def-vl-immdeps vl-maybe-packeddimension
-  :body
-  (if x
-      (vl-packeddimension-immdeps x ans)
-    ans))
+;; (def-vl-immdeps vl-maybe-packeddimension
+;;   :body
+;;   (if x
+;;       (vl-packeddimension-immdeps x ans)
+;;     ans))
 
-(def-vl-immdeps-list vl-packeddimensionlist vl-packeddimension)
+;; (def-vl-immdeps-list vl-packeddimensionlist vl-packeddimension)
 
-(def-vl-immdeps vl-enumbasekind
-  :body
-  (if (stringp x)
-      ;; User-defined type.  The type might be defined at the top-level or it
-      ;; might be defined somewhere else.  It's an ordinary scope item so we
-      ;; can do the ordinary lookup.
-      (vl-immdeps-add-item x ans)
-    ;; Not a user-defined type, so it must be a basic type like logic [3:0] and
-    ;; it has no dependencies
-    ans))
+;; (def-vl-immdeps vl-enumbasekind
+;;   :body
+;;   (if (stringp x)
+;;       ;; User-defined type.  The type might be defined at the top-level or it
+;;       ;; might be defined somewhere else.  It's an ordinary scope item so we
+;;       ;; can do the ordinary lookup.
+;;       (vl-immdeps-add-item x ans)
+;;     ;; Not a user-defined type, so it must be a basic type like logic [3:0] and
+;;     ;; it has no dependencies
+;;     ans))
 
-(def-vl-immdeps vl-enumbasetype
-  :body
-  (b* (((vl-enumbasetype x))
-       (ans (vl-enumbasekind-immdeps x.kind ans))
-       (ans (vl-maybe-packeddimension-immdeps x.dim ans)))
-    ans))
+;; (def-vl-immdeps vl-enumbasetype
+;;   :body
+;;   (b* (((vl-enumbasetype x))
+;;        (ans (vl-enumbasekind-immdeps x.kind ans))
+;;        (ans (vl-maybe-packeddimension-immdeps x.dim ans)))
+;;     ans))
 
-(def-vl-immdeps vl-enumitem
-  :body
-  (b* (((vl-enumitem x))
-       (ans (vl-maybe-range-immdeps x.range ans))
-       (ans (vl-maybe-expr-immdeps x.value ans)))
-    ans))
+;; (def-vl-immdeps vl-enumitem
+;;   :body
+;;   (b* (((vl-enumitem x))
+;;        (ans (vl-maybe-range-immdeps x.range ans))
+;;        (ans (vl-maybe-expr-immdeps x.value ans)))
+;;     ans))
 
-(def-vl-immdeps-list vl-enumitemlist vl-enumitem)
+;; (def-vl-immdeps-list vl-enumitemlist vl-enumitem)
 
 
-(defines vl-datatype-immdeps
-  :flag-local nil
-  :verify-guards nil
+;; (defines vl-datatype-immdeps
+;;   :flag-local nil
+;;   :verify-guards nil
 
-  (define vl-datatype-immdeps ((x   vl-datatype-p)
-                               (ans vl-immdeps-p)
-                               &key
-                               ((ss       vl-scopestack-p)  'ss)
-                               ((ctx      acl2::any-p)      'ctx))
-    :returns (new-ans vl-immdeps-p)
-    :measure (vl-datatype-count x)
-    :flag :datatype
-    (b* ((ans (vl-immdeps-fix ans)))
-      (vl-datatype-case x
-        (:vl-coretype
-         (b* ((ans (vl-packeddimensionlist-immdeps x.pdims ans))
-              (ans (vl-packeddimensionlist-immdeps x.udims ans)))
-           ans))
-        (:vl-struct
-         (b* ((ans (vl-structmemberlist-immdeps x.members ans))
-              (ans (vl-packeddimensionlist-immdeps x.pdims ans))
-              (ans (vl-packeddimensionlist-immdeps x.udims ans)))
-           ans))
-        (:vl-union
-         (b* ((ans (vl-structmemberlist-immdeps x.members ans))
-              (ans (vl-packeddimensionlist-immdeps x.pdims ans))
-              (ans (vl-packeddimensionlist-immdeps x.udims ans)))
-           ans))
-        (:vl-enum
-         (b* ((ans (vl-enumbasetype-immdeps x.basetype ans))
-              (ans (vl-enumitemlist-immdeps x.items ans))
-              (ans (vl-packeddimensionlist-immdeps x.pdims ans))
-              (ans (vl-packeddimensionlist-immdeps x.udims ans)))
-           ans))
-        (:vl-usertype
-         (b* ((ans (vl-scopeexpr-immdeps x.name ans))
-              (ans (vl-packeddimensionlist-immdeps x.pdims ans))
-              (ans (vl-packeddimensionlist-immdeps x.udims ans)))
-           ans)))))
+;;   (define vl-datatype-immdeps ((x   vl-datatype-p)
+;;                                (ans vl-immdeps-p)
+;;                                &key
+;;                                ((ss       vl-scopestack-p)  'ss)
+;;                                ((ctx      acl2::any-p)      'ctx))
+;;     :returns (new-ans vl-immdeps-p)
+;;     :measure (vl-datatype-count x)
+;;     :flag :datatype
+;;     (b* ((ans (vl-immdeps-fix ans)))
+;;       (vl-datatype-case x
+;;         (:vl-coretype
+;;          (b* ((ans (vl-packeddimensionlist-immdeps x.pdims ans))
+;;               (ans (vl-packeddimensionlist-immdeps x.udims ans)))
+;;            ans))
+;;         (:vl-struct
+;;          (b* ((ans (vl-structmemberlist-immdeps x.members ans))
+;;               (ans (vl-packeddimensionlist-immdeps x.pdims ans))
+;;               (ans (vl-packeddimensionlist-immdeps x.udims ans)))
+;;            ans))
+;;         (:vl-union
+;;          (b* ((ans (vl-structmemberlist-immdeps x.members ans))
+;;               (ans (vl-packeddimensionlist-immdeps x.pdims ans))
+;;               (ans (vl-packeddimensionlist-immdeps x.udims ans)))
+;;            ans))
+;;         (:vl-enum
+;;          (b* ((ans (vl-enumbasetype-immdeps x.basetype ans))
+;;               (ans (vl-enumitemlist-immdeps x.items ans))
+;;               (ans (vl-packeddimensionlist-immdeps x.pdims ans))
+;;               (ans (vl-packeddimensionlist-immdeps x.udims ans)))
+;;            ans))
+;;         (:vl-usertype
+;;          (b* ((ans (vl-scopeexpr-immdeps x.name ans))
+;;               (ans (vl-packeddimensionlist-immdeps x.pdims ans))
+;;               (ans (vl-packeddimensionlist-immdeps x.udims ans)))
+;;            ans)))))
 
-  (define vl-structmemberlist-immdeps ((x   vl-structmemberlist-p)
-                                       (ans vl-immdeps-p)
-                                       &key
-                                       ((ss  vl-scopestack-p)  'ss)
-                                       ((ctx acl2::any-p)      'ctx))
-    :returns (new-ans vl-immdeps-p)
-    :measure (vl-structmemberlist-count x)
-    :flag :structmemberlist
-    (b* (((when (atom x))
-          (vl-immdeps-fix ans))
-         (ans (vl-structmember-immdeps (car x) ans)))
-      (vl-structmemberlist-immdeps (cdr x) ans)))
+;;   (define vl-structmemberlist-immdeps ((x   vl-structmemberlist-p)
+;;                                        (ans vl-immdeps-p)
+;;                                        &key
+;;                                        ((ss  vl-scopestack-p)  'ss)
+;;                                        ((ctx acl2::any-p)      'ctx))
+;;     :returns (new-ans vl-immdeps-p)
+;;     :measure (vl-structmemberlist-count x)
+;;     :flag :structmemberlist
+;;     (b* (((when (atom x))
+;;           (vl-immdeps-fix ans))
+;;          (ans (vl-structmember-immdeps (car x) ans)))
+;;       (vl-structmemberlist-immdeps (cdr x) ans)))
 
-  (define vl-structmember-immdeps ((x   vl-structmember-p)
-                                   (ans vl-immdeps-p)
-                                   &key
-                                   ((ss  vl-scopestack-p)  'ss)
-                                   ((ctx acl2::any-p)      'ctx))
-    :returns (new-ans vl-immdeps-p)
-    :flag :structmember
-    :measure (vl-structmember-count x)
-    (b* (((vl-structmember x))
-         (ans (vl-datatype-immdeps x.type ans))
-         (ans (vl-maybe-expr-immdeps x.rhs ans)))
-      ans))
-  ///
-  (verify-guards vl-datatype-immdeps-fn)
-  (deffixequiv-mutual vl-datatype-immdeps))
+;;   (define vl-structmember-immdeps ((x   vl-structmember-p)
+;;                                    (ans vl-immdeps-p)
+;;                                    &key
+;;                                    ((ss  vl-scopestack-p)  'ss)
+;;                                    ((ctx acl2::any-p)      'ctx))
+;;     :returns (new-ans vl-immdeps-p)
+;;     :flag :structmember
+;;     :measure (vl-structmember-count x)
+;;     (b* (((vl-structmember x))
+;;          (ans (vl-datatype-immdeps x.type ans))
+;;          (ans (vl-maybe-expr-immdeps x.rhs ans)))
+;;       ans))
+;;   ///
+;;   (verify-guards vl-datatype-immdeps-fn)
+;;   (deffixequiv-mutual vl-datatype-immdeps))
 
-(def-vl-immdeps vl-maybe-datatype
-  :body
-  (if x
-      (vl-datatype-immdeps x ans)
-    ans))
+;; (def-vl-immdeps vl-maybe-datatype
+;;   :body
+;;   (if x
+;;       (vl-datatype-immdeps x ans)
+;;     ans))
 
 (def-vl-immdeps vl-interfaceport
   :ctxp nil
@@ -509,19 +590,19 @@ elements.")
 (def-vl-immdeps-list vl-portdecllist vl-portdecl :ctxp nil)
 
 
-(def-vl-immdeps vl-gatedelay
-  :body
-  (b* (((vl-gatedelay x))
-       (ans (vl-expr-immdeps x.rise ans))
-       (ans (vl-expr-immdeps x.fall ans))
-       (ans (vl-maybe-expr-immdeps x.high ans)))
-    ans))
+;; (def-vl-immdeps vl-gatedelay
+;;   :body
+;;   (b* (((vl-gatedelay x))
+;;        (ans (vl-expr-immdeps x.rise ans))
+;;        (ans (vl-expr-immdeps x.fall ans))
+;;        (ans (vl-maybe-expr-immdeps x.high ans)))
+;;     ans))
 
-(def-vl-immdeps vl-maybe-gatedelay
-  :body
-  (if x
-      (vl-gatedelay-immdeps x ans)
-    ans))
+;; (def-vl-immdeps vl-maybe-gatedelay
+;;   :body
+;;   (if x
+;;       (vl-gatedelay-immdeps x ans)
+;;     ans))
 
 (def-vl-immdeps vl-assign
   :ctxp nil
@@ -571,55 +652,55 @@ elements.")
 (def-vl-immdeps-list vl-importlist vl-import :ctxp nil)
 
 
-(def-vl-immdeps vl-plainarg
-  :body
-  (b* (((vl-plainarg x)))
-    (vl-maybe-expr-immdeps x.expr ans)))
+;; (def-vl-immdeps vl-plainarg
+;;   :body
+;;   (b* (((vl-plainarg x)))
+;;     (vl-maybe-expr-immdeps x.expr ans)))
 
-(def-vl-immdeps-list vl-plainarglist vl-plainarg)
+;; (def-vl-immdeps-list vl-plainarglist vl-plainarg)
 
-(def-vl-immdeps vl-namedarg
-  :body
-  (b* (((vl-namedarg x)))
-    (vl-maybe-expr-immdeps x.expr ans)))
+;; (def-vl-immdeps vl-namedarg
+;;   :body
+;;   (b* (((vl-namedarg x)))
+;;     (vl-maybe-expr-immdeps x.expr ans)))
 
-(def-vl-immdeps-list vl-namedarglist vl-namedarg)
+;; (def-vl-immdeps-list vl-namedarglist vl-namedarg)
 
-(def-vl-immdeps vl-arguments
-  :body
-  (vl-arguments-case x
-    (:vl-arguments-plain (vl-plainarglist-immdeps x.args ans))
-    (:vl-arguments-named (vl-namedarglist-immdeps x.args ans))))
+;; (def-vl-immdeps vl-arguments
+;;   :body
+;;   (vl-arguments-case x
+;;     (:vl-arguments-plain (vl-plainarglist-immdeps x.args ans))
+;;     (:vl-arguments-named (vl-namedarglist-immdeps x.args ans))))
 
-(def-vl-immdeps-list vl-argumentlist vl-arguments)
+;; (def-vl-immdeps-list vl-argumentlist vl-arguments)
 
-(def-vl-immdeps vl-paramvalue
-  :body
-  (vl-paramvalue-case x
-    :expr (vl-expr-immdeps x.expr ans)
-    :type (vl-datatype-immdeps x.type ans)))
+;; (def-vl-immdeps vl-paramvalue
+;;   :body
+;;   (vl-paramvalue-case x
+;;     :expr (vl-expr-immdeps x.expr ans)
+;;     :type (vl-datatype-immdeps x.type ans)))
 
-(def-vl-immdeps-list vl-paramvaluelist vl-paramvalue)
+;; (def-vl-immdeps-list vl-paramvaluelist vl-paramvalue)
 
-(def-vl-immdeps vl-maybe-paramvalue
-  :body
-  (if x
-      (vl-paramvalue-immdeps x ans)
-    ans))
+;; (def-vl-immdeps vl-maybe-paramvalue
+;;   :body
+;;   (if x
+;;       (vl-paramvalue-immdeps x ans)
+;;     ans))
 
 
-(def-vl-immdeps vl-namedparamvalue
-  :body
-  (b* (((vl-namedparamvalue x)))
-    (vl-maybe-paramvalue-immdeps x.value ans)))
+;; (def-vl-immdeps vl-namedparamvalue
+;;   :body
+;;   (b* (((vl-namedparamvalue x)))
+;;     (vl-maybe-paramvalue-immdeps x.value ans)))
 
-(def-vl-immdeps-list vl-namedparamvaluelist vl-namedparamvalue)
+;; (def-vl-immdeps-list vl-namedparamvaluelist vl-namedparamvalue)
 
-(def-vl-immdeps vl-paramargs
-  :body
-  (vl-paramargs-case x
-    (:vl-paramargs-plain (vl-paramvaluelist-immdeps x.args ans))
-    (:vl-paramargs-named (vl-namedparamvaluelist-immdeps x.args ans))))
+;; (def-vl-immdeps vl-paramargs
+;;   :body
+;;   (vl-paramargs-case x
+;;     (:vl-paramargs-plain (vl-paramvaluelist-immdeps x.args ans))
+;;     (:vl-paramargs-named (vl-namedparamvaluelist-immdeps x.args ans))))
 
 (def-vl-immdeps vl-modinst
   :ctxp nil
@@ -647,19 +728,19 @@ elements.")
 
 (def-vl-immdeps-list vl-gateinstlist vl-gateinst :ctxp nil)
 
-(def-vl-immdeps vl-paramtype
-  :body
-  (vl-paramtype-case x
-    (:vl-implicitvalueparam
-     (b* ((ans (vl-maybe-range-immdeps x.range ans))
-          (ans (vl-maybe-expr-immdeps x.default ans)))
-       ans))
-    (:vl-explicitvalueparam
-     (b* ((ans (vl-datatype-immdeps x.type ans))
-          (ans (vl-maybe-expr-immdeps x.default ans)))
-       ans))
-    (:vl-typeparam
-     (vl-maybe-datatype-immdeps x.default ans))))
+;; (def-vl-immdeps vl-paramtype
+;;   :body
+;;   (vl-paramtype-case x
+;;     (:vl-implicitvalueparam
+;;      (b* ((ans (vl-maybe-range-immdeps x.range ans))
+;;           (ans (vl-maybe-expr-immdeps x.default ans)))
+;;        ans))
+;;     (:vl-explicitvalueparam
+;;      (b* ((ans (vl-datatype-immdeps x.type ans))
+;;           (ans (vl-maybe-expr-immdeps x.default ans)))
+;;        ans))
+;;     (:vl-typeparam
+;;      (vl-maybe-datatype-immdeps x.default ans))))
 
 (def-vl-immdeps vl-paramdecl
   :ctxp nil
@@ -670,176 +751,176 @@ elements.")
 
 (def-vl-immdeps-list vl-paramdecllist vl-paramdecl :ctxp nil)
 
-(def-vl-immdeps vl-evatom
-  :body
-  (b* (((vl-evatom x)))
-    (vl-expr-immdeps x.expr ans)))
+;; (def-vl-immdeps vl-evatom
+;;   :body
+;;   (b* (((vl-evatom x)))
+;;     (vl-expr-immdeps x.expr ans)))
 
-(def-vl-immdeps-list vl-evatomlist vl-evatom)
+;; (def-vl-immdeps-list vl-evatomlist vl-evatom)
 
-(def-vl-immdeps vl-eventcontrol
-  :body
-  (b* (((vl-eventcontrol x)))
-    (vl-evatomlist-immdeps x.atoms ans)))
+;; (def-vl-immdeps vl-eventcontrol
+;;   :body
+;;   (b* (((vl-eventcontrol x)))
+;;     (vl-evatomlist-immdeps x.atoms ans)))
 
-(def-vl-immdeps vl-delaycontrol
-  :body
-  (b* (((vl-delaycontrol x)))
-    (vl-expr-immdeps x.value ans)))
+;; (def-vl-immdeps vl-delaycontrol
+;;   :body
+;;   (b* (((vl-delaycontrol x)))
+;;     (vl-expr-immdeps x.value ans)))
 
-(def-vl-immdeps vl-repeateventcontrol
-  :body
-  (b* (((vl-repeateventcontrol x))
-       (ans (vl-expr-immdeps x.expr ans))
-       (ans (vl-eventcontrol-immdeps x.ctrl ans)))
-    ans))
+;; (def-vl-immdeps vl-repeateventcontrol
+;;   :body
+;;   (b* (((vl-repeateventcontrol x))
+;;        (ans (vl-expr-immdeps x.expr ans))
+;;        (ans (vl-eventcontrol-immdeps x.ctrl ans)))
+;;     ans))
 
-(def-vl-immdeps vl-delayoreventcontrol
-  :body
-  (case (tag x)
-    (:vl-delaycontrol (vl-delaycontrol-immdeps x ans))
-    (:vl-eventcontrol (vl-eventcontrol-immdeps x ans))
-    (otherwise        (vl-repeateventcontrol-immdeps x ans))))
+;; (def-vl-immdeps vl-delayoreventcontrol
+;;   :body
+;;   (case (tag x)
+;;     (:vl-delaycontrol (vl-delaycontrol-immdeps x ans))
+;;     (:vl-eventcontrol (vl-eventcontrol-immdeps x ans))
+;;     (otherwise        (vl-repeateventcontrol-immdeps x ans))))
 
-(def-vl-immdeps vl-maybe-delayoreventcontrol
-  :body
-  (if x
-      (vl-delayoreventcontrol-immdeps x ans)
-    ans))
-
-
-(defines vl-stmt-immdeps
-  :flag-local nil
-  :verify-guards nil
-  :returns-hints ((and stable-under-simplificationp
-                       '(:expand ((vl-stmt-immdeps x ans)
-                                  (vl-stmtlist-immdeps x ans)
-                                  (vl-caselist-immdeps x ans)))))
+;; (def-vl-immdeps vl-maybe-delayoreventcontrol
+;;   :body
+;;   (if x
+;;       (vl-delayoreventcontrol-immdeps x ans)
+;;     ans))
 
 
-  (define vl-stmt-immdeps ((x   vl-stmt-p)
-                           (ans vl-immdeps-p)
-                           &key
-                           ((ss vl-scopestack-p) 'ss))
-    :returns (new-ans vl-immdeps-p)
-    :measure (vl-stmt-count x)
-    :flag :stmt
-    (b* ((x   (vl-stmt-fix x))
-         (ans (vl-immdeps-fix ans))
-         (ctx x))
-      (vl-stmt-case x
-        (:vl-nullstmt
-         ans)
-        (:vl-assignstmt
-         (b* ((ans (vl-expr-immdeps x.lvalue ans))
-              (ans (vl-expr-immdeps x.expr ans))
-              (ans (vl-maybe-delayoreventcontrol-immdeps x.ctrl ans)))
-           ans))
-        (:vl-deassignstmt
-         (vl-expr-immdeps x.lvalue ans))
-        (:vl-enablestmt
-         (b* ((ans (vl-expr-immdeps x.id ans))
-              (ans (vl-exprlist-immdeps x.args ans)))
-           ans))
-        (:vl-disablestmt
-         (vl-expr-immdeps x.id ans))
-        (:vl-returnstmt
-         (if x.val (vl-expr-immdeps x.val ans) ans))
-        (:vl-eventtriggerstmt
-         (vl-expr-immdeps x.id ans))
-        (:vl-casestmt
-         (b* ((ans (vl-expr-immdeps x.test ans))
-              (ans (vl-caselist-immdeps x.caselist ans))
-              (ans (vl-stmt-immdeps x.default ans)))
-           ans))
-        (:vl-ifstmt
-         (b* ((ans (vl-expr-immdeps x.condition ans))
-              (ans (vl-stmt-immdeps x.truebranch ans))
-              (ans (vl-stmt-immdeps x.falsebranch ans)))
-           ans))
-        (:vl-foreverstmt
-         (vl-stmt-immdeps x.body ans))
-        (:vl-waitstmt
-         (b* ((ans (vl-expr-immdeps x.condition ans))
-              (ans (vl-stmt-immdeps x.body ans)))
-           ans))
-        (:vl-repeatstmt
-         (b* ((ans (vl-expr-immdeps x.condition ans))
-              (ans (vl-stmt-immdeps x.body ans)))
-           ans))
-        (:vl-whilestmt
-         (b* ((ans (vl-expr-immdeps x.condition ans))
-              (ans (vl-stmt-immdeps x.body ans)))
-           ans))
-        (:vl-forstmt
-         (b* ((ans (vl-vardecllist-immdeps x.initdecls ans))
-              (ans (vl-stmtlist-immdeps x.initassigns ans))
-              (ans (vl-expr-immdeps x.test ans))
-              (ans (vl-stmtlist-immdeps x.stepforms ans))
-              (ans (vl-stmt-immdeps x.body ans)))
-           ans))
-        (:vl-blockstmt
-         (b* ((ss (vl-scopestack-push (vl-blockstmt->blockscope x) ss))
-              (ans (vl-importlist-immdeps x.imports ans))
-              (ans (vl-paramdecllist-immdeps x.paramdecls ans))
-              (ans (vl-vardecllist-immdeps x.vardecls ans))
-              (ans (vl-stmtlist-immdeps x.stmts ans)))
-           ans))
-        (:vl-timingstmt
-         (b* ((ans (vl-delayoreventcontrol-immdeps x.ctrl ans))
-              (ans (vl-stmt-immdeps x.body ans)))
-           ans)))))
+;; (defines vl-stmt-immdeps
+;;   :flag-local nil
+;;   :verify-guards nil
+;;   :returns-hints ((and stable-under-simplificationp
+;;                        '(:expand ((vl-stmt-immdeps x ans)
+;;                                   (vl-stmtlist-immdeps x ans)
+;;                                   (vl-caselist-immdeps x ans)))))
 
-  (define vl-stmtlist-immdeps ((x   vl-stmtlist-p)
-                               (ans vl-immdeps-p)
-                               &key
-                               ((ss vl-scopestack-p) 'ss))
-    :returns (new-ans vl-immdeps-p)
-    :measure (vl-stmtlist-count x)
-    :flag :stmtlist
-    (b* ((x   (vl-stmtlist-fix x))
-         (ans (vl-immdeps-fix ans))
-         ((when (atom x))
-          ans)
-         (ans (vl-stmt-immdeps (car x) ans)))
-      (vl-stmtlist-immdeps (cdr x) ans)))
 
-  (define vl-caselist-immdeps ((x   vl-caselist-p)
-                               (ans vl-immdeps-p)
-                               &key
-                               ((ss       vl-scopestack-p)  'ss)
-                               ((ctx      acl2::any-p)      'ctx))
-    :returns (new-ans vl-immdeps-p)
-    :flag :caselist
-    :measure (vl-caselist-count x)
-    (b* ((x   (vl-caselist-fix x))
-         (ans (vl-immdeps-fix ans))
-         ((when (atom x))
-          ans)
-         ((cons exprs1 body1) (car x))
-         (ans (vl-exprlist-immdeps exprs1 ans))
-         (ans (vl-stmt-immdeps body1 ans)))
-      (vl-caselist-immdeps (cdr x) ans)))
+;;   (define vl-stmt-immdeps ((x   vl-stmt-p)
+;;                            (ans vl-immdeps-p)
+;;                            &key
+;;                            ((ss vl-scopestack-p) 'ss))
+;;     :returns (new-ans vl-immdeps-p)
+;;     :measure (vl-stmt-count x)
+;;     :flag :stmt
+;;     (b* ((x   (vl-stmt-fix x))
+;;          (ans (vl-immdeps-fix ans))
+;;          (ctx x))
+;;       (vl-stmt-case x
+;;         (:vl-nullstmt
+;;          ans)
+;;         (:vl-assignstmt
+;;          (b* ((ans (vl-expr-immdeps x.lvalue ans))
+;;               (ans (vl-expr-immdeps x.expr ans))
+;;               (ans (vl-maybe-delayoreventcontrol-immdeps x.ctrl ans)))
+;;            ans))
+;;         (:vl-deassignstmt
+;;          (vl-expr-immdeps x.lvalue ans))
+;;         (:vl-enablestmt
+;;          (b* ((ans (vl-expr-immdeps x.id ans))
+;;               (ans (vl-exprlist-immdeps x.args ans)))
+;;            ans))
+;;         (:vl-disablestmt
+;;          (vl-expr-immdeps x.id ans))
+;;         (:vl-returnstmt
+;;          (if x.val (vl-expr-immdeps x.val ans) ans))
+;;         (:vl-eventtriggerstmt
+;;          (vl-expr-immdeps x.id ans))
+;;         (:vl-casestmt
+;;          (b* ((ans (vl-expr-immdeps x.test ans))
+;;               (ans (vl-caselist-immdeps x.caselist ans))
+;;               (ans (vl-stmt-immdeps x.default ans)))
+;;            ans))
+;;         (:vl-ifstmt
+;;          (b* ((ans (vl-expr-immdeps x.condition ans))
+;;               (ans (vl-stmt-immdeps x.truebranch ans))
+;;               (ans (vl-stmt-immdeps x.falsebranch ans)))
+;;            ans))
+;;         (:vl-foreverstmt
+;;          (vl-stmt-immdeps x.body ans))
+;;         (:vl-waitstmt
+;;          (b* ((ans (vl-expr-immdeps x.condition ans))
+;;               (ans (vl-stmt-immdeps x.body ans)))
+;;            ans))
+;;         (:vl-repeatstmt
+;;          (b* ((ans (vl-expr-immdeps x.condition ans))
+;;               (ans (vl-stmt-immdeps x.body ans)))
+;;            ans))
+;;         (:vl-whilestmt
+;;          (b* ((ans (vl-expr-immdeps x.condition ans))
+;;               (ans (vl-stmt-immdeps x.body ans)))
+;;            ans))
+;;         (:vl-forstmt
+;;          (b* ((ans (vl-vardecllist-immdeps x.initdecls ans))
+;;               (ans (vl-stmtlist-immdeps x.initassigns ans))
+;;               (ans (vl-expr-immdeps x.test ans))
+;;               (ans (vl-stmtlist-immdeps x.stepforms ans))
+;;               (ans (vl-stmt-immdeps x.body ans)))
+;;            ans))
+;;         (:vl-blockstmt
+;;          (b* ((ss (vl-scopestack-push (vl-blockstmt->blockscope x) ss))
+;;               (ans (vl-importlist-immdeps x.imports ans))
+;;               (ans (vl-paramdecllist-immdeps x.paramdecls ans))
+;;               (ans (vl-vardecllist-immdeps x.vardecls ans))
+;;               (ans (vl-stmtlist-immdeps x.stmts ans)))
+;;            ans))
+;;         (:vl-timingstmt
+;;          (b* ((ans (vl-delayoreventcontrol-immdeps x.ctrl ans))
+;;               (ans (vl-stmt-immdeps x.body ans)))
+;;            ans)))))
 
-  ///
-  (local (set-default-hints
-          '((and stable-under-simplificationp
-                 '(:expand ((:free (ss ans) (vl-stmt-immdeps x ans))
-                            (:free (ss ans) (vl-stmt-immdeps (vl-stmt-fix x) ans))
-                            (:free (ss ans) (vl-stmtlist-immdeps x ans))
-                            (:free (ss ans) (vl-stmtlist-immdeps (vl-stmtlist-fix x) ans))
-                            (:free (ss ans ctx) (vl-caselist-immdeps x ans))
-                            (:free (ss ans ctx) (vl-caselist-immdeps (vl-caselist-fix x) ans))))))))
+;;   (define vl-stmtlist-immdeps ((x   vl-stmtlist-p)
+;;                                (ans vl-immdeps-p)
+;;                                &key
+;;                                ((ss vl-scopestack-p) 'ss))
+;;     :returns (new-ans vl-immdeps-p)
+;;     :measure (vl-stmtlist-count x)
+;;     :flag :stmtlist
+;;     (b* ((x   (vl-stmtlist-fix x))
+;;          (ans (vl-immdeps-fix ans))
+;;          ((when (atom x))
+;;           ans)
+;;          (ans (vl-stmt-immdeps (car x) ans)))
+;;       (vl-stmtlist-immdeps (cdr x) ans)))
 
-  (deffixequiv-mutual vl-stmt-immdeps)
-  (verify-guards vl-stmt-immdeps-fn))
+;;   (define vl-caselist-immdeps ((x   vl-caselist-p)
+;;                                (ans vl-immdeps-p)
+;;                                &key
+;;                                ((ss       vl-scopestack-p)  'ss)
+;;                                ((ctx      acl2::any-p)      'ctx))
+;;     :returns (new-ans vl-immdeps-p)
+;;     :flag :caselist
+;;     :measure (vl-caselist-count x)
+;;     (b* ((x   (vl-caselist-fix x))
+;;          (ans (vl-immdeps-fix ans))
+;;          ((when (atom x))
+;;           ans)
+;;          ((cons exprs1 body1) (car x))
+;;          (ans (vl-exprlist-immdeps exprs1 ans))
+;;          (ans (vl-stmt-immdeps body1 ans)))
+;;       (vl-caselist-immdeps (cdr x) ans)))
+
+;;   ///
+;;   (local (set-default-hints
+;;           '((and stable-under-simplificationp
+;;                  '(:expand ((:free (ss ans) (vl-stmt-immdeps x ans))
+;;                             (:free (ss ans) (vl-stmt-immdeps (vl-stmt-fix x) ans))
+;;                             (:free (ss ans) (vl-stmtlist-immdeps x ans))
+;;                             (:free (ss ans) (vl-stmtlist-immdeps (vl-stmtlist-fix x) ans))
+;;                             (:free (ss ans ctx) (vl-caselist-immdeps x ans))
+;;                             (:free (ss ans ctx) (vl-caselist-immdeps (vl-caselist-fix x) ans))))))))
+
+;;   (deffixequiv-mutual vl-stmt-immdeps)
+;;   (verify-guards vl-stmt-immdeps-fn))
 
 
 (def-vl-immdeps vl-always
   :ctxp nil
   :body
   (b* (((vl-always x)))
-    (vl-stmt-immdeps x.stmt ans)))
+    (vl-stmt-immdeps x.stmt ans :ctx x)))
 
 (def-vl-immdeps-list vl-alwayslist vl-always :ctxp nil)
 
@@ -847,7 +928,7 @@ elements.")
   :ctxp nil
   :body
   (b* (((vl-initial x)))
-    (vl-stmt-immdeps x.stmt ans)))
+    (vl-stmt-immdeps x.stmt ans :ctx x)))
 
 (def-vl-immdeps-list vl-initiallist vl-initial :ctxp nil)
 
@@ -867,7 +948,7 @@ elements.")
        (ans (vl-importlist-immdeps x.imports ans))
        (ans (vl-paramdecllist-immdeps x.paramdecls ans))
        (ans (vl-vardecllist-immdeps x.vardecls ans)))
-    (vl-stmt-immdeps x.body ans)))
+    (vl-stmt-immdeps x.body ans :ctx x)))
 
 (def-vl-immdeps-list vl-fundecllist vl-fundecl :ctxp nil)
 
@@ -881,7 +962,7 @@ elements.")
        (ans (vl-importlist-immdeps x.imports ans))
        (ans (vl-paramdecllist-immdeps x.paramdecls ans))
        (ans (vl-vardecllist-immdeps x.vardecls ans)))
-    (vl-stmt-immdeps x.body ans)))
+    (vl-stmt-immdeps x.body ans :ctx x)))
 
 (def-vl-immdeps-list vl-taskdecllist vl-taskdecl :ctxp nil)
 
